Weidenbach_Book/IsaSAT/IsaSAT_Backtrack_LLVM.thy
@@ -19,44 +19,6 @@ sepref_def update_lbd_and_mark_used_impl
   apply (annot_unat_const \<open>TYPE(32)\<close>)
   by sepref
 
-lemma mop_mark_added_heur_st_alt_def:
-  \<open>mop_mark_added_heur_st L S = do {
-  let (heur, S) = extract_heur_wl_heur S;
-  heur \<leftarrow> mop_mark_added_heur L True heur;
-  RETURN (update_heur_wl_heur heur S)
-  }\<close>
-  unfolding mop_mark_added_heur_st_def
-  by (auto simp: incr_restart_stat_def state_extractors split: isasat_int_splits
-    intro!: ext)
-
-sepref_def mop_mark_added_heur_iml
-  is \<open>uncurry2 mop_mark_added_heur\<close>
-  :: \<open>atom_assn\<^sup>k *\<^sub>a bool1_assn\<^sup>k *\<^sub>a heuristic_assn\<^sup>d \<rightarrow>\<^sub>a heuristic_assn\<close>
-  supply [sepref_fr_rules] = mark_added_heur_impl_refine
-  unfolding mop_mark_added_heur_def
-  by sepref
-
-sepref_register mop_mark_added_heur mop_mark_added_heur_st mark_added_clause_heur2 maybe_mark_added_clause_heur2
-
-sepref_def mop_mark_added_heur_st_impl
-  is \<open>uncurry mop_mark_added_heur_st\<close>
-  :: \<open>atom_assn\<^sup>k *\<^sub>a isasat_bounded_assn\<^sup>d \<rightarrow>\<^sub>a isasat_bounded_assn\<close>
-  unfolding mop_mark_added_heur_st_alt_def
-  by sepref
-
-sepref_def mark_added_clause_heur2_impl
-  is \<open>uncurry mark_added_clause_heur2\<close>
-  :: \<open>isasat_bounded_assn\<^sup>d *\<^sub>a sint64_nat_assn\<^sup>k \<rightarrow>\<^sub>a isasat_bounded_assn\<close>
-  unfolding mark_added_clause_heur2_def
-  apply (annot_snat_const \<open>TYPE(64)\<close>)
-  by sepref
-
-sepref_def maybe_mark_added_clause_heur2_impl
-  is \<open>uncurry maybe_mark_added_clause_heur2\<close>
-  :: \<open>isasat_bounded_assn\<^sup>d *\<^sub>a sint64_nat_assn\<^sup>k \<rightarrow>\<^sub>a isasat_bounded_assn\<close>
-  unfolding maybe_mark_added_clause_heur2_def
-  by sepref
-
 lemma isa_empty_conflict_and_extract_clause_heur_alt_def:
     \<open>isa_empty_conflict_and_extract_clause_heur M D outl = do {
      let C = replicate (length outl) (outl!0);
